examples/Hoare/Verify.v
@@ -49,8 +49,8 @@ Module ImpVerify (I : ImpLang).
   Local Existing Instance RTypeOk_typ.
   Local Existing Instance Typ2_Fun.
   Local Existing Instance Typ2Ok_Fun.
-  Local Existing Instance ModularTypes.Typ0_Prop.
-  Local Existing Instance ModularTypes.Typ0Ok_Prop.
+  Local Existing Instance CoreTypes.Typ0_Prop.
+  Local Existing Instance CoreTypes.Typ0Ok_Prop.
 
   Section with_fs.
     Variable fs' : SymEnv.functions typ _.
@@ -448,11 +448,11 @@ Module ImpVerify (I : ImpLang).
         Ptrns.ptrn_elim. subst. subst.
         generalize dependent (AppN.apps e es); intros; subst.
         destruct x; simpl in *.
-        assert (t = ModularTypes.tyBase0 tyValue).
+        assert (t = CoreTypes.tyBase0 tyValue).
         { autorewrite with exprD_rw in H0.
           cbn in H0.
-          destruct (ModularTypes.mtyp_cast tsym _ t
-                     (ModularTypes.tyBase0 tyValue)). auto. inversion H0. }
+          destruct (CoreTypes.ctyp_cast tsym _ t
+                     (CoreTypes.tyBase0 tyValue)). auto. inversion H0. }
         subst. cbn in H0.
         inv_all. subst.
         cbn. eexists; split; eauto. }
@@ -598,20 +598,20 @@ Module ImpVerify (I : ImpLang).
           let resultV := eval vm_compute in result in
           lazymatch resultV with
           | Solved _ =>
-            change (@propD _ _ _ (@ModularTypes.Typ0_Prop _ _) (Expr_expr tbl) nil nil g) ;
+            change (@propD _ _ _ (@CoreTypes.Typ0_Prop _ _) (Expr_expr tbl) nil nil g) ;
               cut(result = resultV) ;
               [ exact (@rtac_Solved_closed_soundness _ _ _ _ _ _ (tac_sound tbl) nil nil g)
               | vm_cast_no_check (@eq_refl _ resultV) ]
           | More_ _ ?g' =>
             pose (g'V := g') ;
-            let post := constr:(match @goalD _ _ _ (@ModularTypes.Typ0_Prop _ _) (Expr_expr tbl) nil nil g'V with
+            let post := constr:(match @goalD _ _ _ (@CoreTypes.Typ0_Prop _ _) (Expr_expr tbl) nil nil g'V with
                                 | Some G => G HList.Hnil HList.Hnil
                                 | None => True
                                 end) in
             let post := reduce_propD tbl g'V post in
             let G := post in
             cut G ;
-              [ change (@closedD _ _ _ (@ModularTypes.Typ0_Prop _ _) (Expr_expr tbl) nil nil g g'V) ;
+              [ change (@closedD _ _ _ (@CoreTypes.Typ0_Prop _ _) (Expr_expr tbl) nil nil g g'V) ;
                 cut (result = More_ (@TopSubst _ _ _ _) g'V) ;
                 [ exact (@rtac_More_closed_soundness _ _ _ _ _ _ (tac_sound tbl) nil nil g g'V)
                 | vm_cast_no_check (@eq_refl _ resultV) ]
@@ -753,7 +753,7 @@ Definition PHASE3_tauto : imp_tac :=
   (*
 Fixpoint parse_ands (e : expr typ func) : list (expr typ func) :=
   match e with
-    | App (App (Inj (inr (ILogicFunc.ilf_and (ModularTypestyBase0 tyProp)))) P) Q =>
+    | App (App (Inj (inr (ILogicFunc.ilf_and (CoreTypestyBase0 tyProp)))) P) Q =>
       parse_ands P ++ parse_ands Q
     | _ => e :: nil
   end.
