theories/CTypes/BaseType.v
@@ -4,7 +4,7 @@ Require Import MirrorCore.TypesI.
 Require Import MirrorCore.Views.FuncView.
 Require Import MirrorCore.Views.Ptrns.
 Require Import MirrorCore.Views.TypeView.
-Require Import MirrorCore.MTypes.ModularTypes.
+Require Import MirrorCore.CTypes.CoreTypes.
 Require Import MirrorCore.Reify.ReifyClass.
 
 Require Import ExtLib.Core.RelDec.
